Given_Clause_Loops/Fair_Zipperposition_Loop_without_Ghosts.thy
@@ -12,38 +12,118 @@ begin
 
 subsection \<open>Locale\<close>
 
-type_synonym ('t, 'p, 'f) fair_ZL_state = "'t \<times> 'p \<times> 'f option \<times> 'f fset"
+type_synonym ('t, 'p, 'f) fair_ZL_state_wo_ghosts = "'t \<times> 'p \<times> 'f option \<times> 'f fset"
 
-context fair_zipperposition_loop
+locale fair_zipperposition_loop_wo_ghosts =
+  w_ghosts?: fair_zipperposition_loop Bot_F Inf_F Bot_G Q entails_q Inf_G_q Red_I_q Red_F_q \<G>_F_q
+    \<G>_I_q Equiv_F Prec_F t_empty t_select t_add t_remove t_felems p_empty p_select p_add p_remove
+    p_felems Prec_S
+  for
+    Bot_F :: "'f set" and
+    Inf_F :: "'f inference set" and
+    Bot_G :: "'g set" and
+    Q :: "'q set" and
+    entails_q :: "'q \<Rightarrow> 'g set \<Rightarrow> 'g set \<Rightarrow> bool" and
+    Inf_G_q :: "'q \<Rightarrow> 'g inference set" and
+    Red_I_q :: "'q \<Rightarrow> 'g set \<Rightarrow> 'g inference set" and
+    Red_F_q :: "'q \<Rightarrow> 'g set \<Rightarrow> 'g set" and
+    \<G>_F_q :: "'q \<Rightarrow> 'f \<Rightarrow> 'g set" and
+    \<G>_I_q :: "'q \<Rightarrow> 'f inference \<Rightarrow> 'g inference set option" and
+    Equiv_F :: "'f \<Rightarrow> 'f \<Rightarrow> bool" (infix "\<doteq>" 50) and
+    Prec_F :: "'f \<Rightarrow> 'f \<Rightarrow> bool" (infix "\<prec>\<cdot>" 50) and
+    t_empty :: "'t" and
+    t_select :: "'t \<Rightarrow> 'f inference llist" and
+    t_add :: "'f inference llist \<Rightarrow> 't \<Rightarrow> 't" and
+    t_remove :: "'f inference llist \<Rightarrow> 't \<Rightarrow> 't" and
+    t_felems :: "'t \<Rightarrow> 'f inference llist fset" and
+    p_empty :: "'p" and
+    p_select :: "'p \<Rightarrow> 'f" and
+    p_add :: "'f \<Rightarrow> 'p \<Rightarrow> 'p" and
+    p_remove :: "'f \<Rightarrow> 'p \<Rightarrow> 'p" and
+    p_felems :: "'p \<Rightarrow> 'f fset" and
+    Prec_S :: "'f \<Rightarrow> 'f \<Rightarrow> bool" (infix "\<prec>S" 50)
 begin
 
 inductive
-  fair_ZL_without_ghosts :: "('t, 'p, 'f) fair_ZL_state \<Rightarrow> ('t, 'p, 'f) fair_ZL_state \<Rightarrow> bool"
-  (infix "\<leadsto>ZLf" 50)
+  fair_ZL_wo_ghosts ::
+  "('t, 'p, 'f) fair_ZL_state_wo_ghosts \<Rightarrow> ('t, 'p, 'f) fair_ZL_state_wo_ghosts \<Rightarrow> bool"
+  (infix "\<leadsto>ZLfw" 50)
 where
   compute_infer: "T \<noteq> t_empty \<Longrightarrow> t_select T = LCons \<iota>0 \<iota>s \<Longrightarrow>
     \<iota>0 \<in> no_labels.Red_I (fset A \<union> {C}) \<Longrightarrow>
-    (T, P, None, A) \<leadsto>ZLf (t_add \<iota>s (t_remove (t_select T) T), p_add C P, None, A)"
+    (T, P, None, A) \<leadsto>ZLfw (t_add \<iota>s (t_remove (t_select T) T), p_add C P, None, A)"
 | choose_p: "P \<noteq> p_empty \<Longrightarrow>
-    (T, P, None, A) \<leadsto>ZLf (T, p_remove (p_select P) P, Some (p_select P), A)"
+    (T, P, None, A) \<leadsto>ZLfw (T, p_remove (p_select P) P, Some (p_select P), A)"
 | delete_fwd: "C \<in> no_labels.Red_F (fset A) \<or> (\<exists>C' \<in> fset A. C' \<preceq>\<cdot> C) \<Longrightarrow>
-    (T, P, Some C, A) \<leadsto>ZLf (T, P, None, A)"
+    (T, P, Some C, A) \<leadsto>ZLfw (T, P, None, A)"
 | simplify_fwd: "C' \<prec>S C \<Longrightarrow> C \<in> no_labels.Red_F (fset A \<union> {C'}) \<Longrightarrow>
-    (T, P, Some C, A) \<leadsto>ZLf (T, P, Some C', A)"
+    (T, P, Some C, A) \<leadsto>ZLfw (T, P, Some C', A)"
 | delete_bwd: "C' |\<notin>| A \<Longrightarrow> C' \<in> no_labels.Red_F {C} \<or> C' \<cdot>\<succ> C \<Longrightarrow>
-    (T, P, Some C, A |\<union>| {|C'|}) \<leadsto>ZLf (T, P, Some C, A)"
+    (T, P, Some C, A |\<union>| {|C'|}) \<leadsto>ZLfw (T, P, Some C, A)"
 | simplify_bwd: "C' |\<notin>| A \<Longrightarrow> C'' \<prec>S C' \<Longrightarrow> C' \<in> no_labels.Red_F {C, C''} \<Longrightarrow>
-    (T, P, Some C, A |\<union>| {|C'|}) \<leadsto>ZLf (T, p_add C'' P, Some C, A)"
+    (T, P, Some C, A |\<union>| {|C'|}) \<leadsto>ZLfw (T, p_add C'' P, Some C, A)"
 | schedule_infer: "flat_inferences_of (set \<iota>ss) = no_labels.Inf_between (fset A) {C} \<Longrightarrow>
-    (T, P, Some C, A) \<leadsto>ZLf (fold t_add \<iota>ss T, P, None, A |\<union>| {|C|})"
+    (T, P, Some C, A) \<leadsto>ZLfw (fold t_add \<iota>ss T, P, None, A |\<union>| {|C|})"
 | delete_orphan_infers: "\<iota>s \<in> todo.elems T \<Longrightarrow> lset \<iota>s \<inter> no_labels.Inf_from (fset A) = {} \<Longrightarrow>
-    (T, P, Y, A) \<leadsto>ZLf (t_remove \<iota>s T, P, Y, A)"
+    (T, P, Y, A) \<leadsto>ZLfw (t_remove \<iota>s T, P, Y, A)"
+
+inductive
+  compute_infer_step ::
+  "('t, 'p, 'f) fair_ZL_state_wo_ghosts \<Rightarrow> ('t, 'p, 'f) fair_ZL_state_wo_ghosts \<Rightarrow> bool"
+where
+  "T \<noteq> t_empty \<Longrightarrow> t_select T = LCons \<iota>0 \<iota>s \<Longrightarrow> \<iota>0 \<in> no_labels.Red_I (fset A \<union> {C}) \<Longrightarrow>
+   compute_infer_step (T, P, None, A)
+     (t_add \<iota>s (t_remove (t_select T) T), p_add C P, None, A)"
+
+inductive
+  choose_p_step ::
+  "('t, 'p, 'f) fair_ZL_state_wo_ghosts \<Rightarrow> ('t, 'p, 'f) fair_ZL_state_wo_ghosts \<Rightarrow> bool"
+where
+  "P \<noteq> p_empty \<Longrightarrow>
+   choose_p_step (T, P, None, A) (T, p_remove (p_select P) P, Some (p_select P), A)"
+
+
+subsection \<open>Definitions and Lemmas\<close>
+
+abbreviation todo_of :: "('t, 'p, 'f) fair_ZL_state_wo_ghosts \<Rightarrow> 't" where
+  "todo_of St \<equiv> fst St"
+abbreviation passive_of :: "('t, 'p, 'f) fair_ZL_state_wo_ghosts \<Rightarrow> 'p" where
+  "passive_of St \<equiv> fst (snd St)"
+abbreviation yy_of :: "('t, 'p, 'f) fair_ZL_state_wo_ghosts \<Rightarrow> 'f option" where
+  "yy_of St \<equiv> fst (snd (snd St))"
+abbreviation active_of :: "('t, 'p, 'f) fair_ZL_state_wo_ghosts \<Rightarrow> 'f fset" where
+  "active_of St \<equiv> snd (snd (snd St))"
+
+abbreviation all_formulas_of :: "('t, 'p, 'f) fair_ZL_state_wo_ghosts \<Rightarrow> 'f set" where
+  "all_formulas_of St \<equiv> passive.elems (passive_of St) \<union> set_option (yy_of St) \<union> fset (active_of St)"
+
+definition
+  Liminf_zl_fstate :: "('t, 'p, 'f) fair_ZL_state_wo_ghosts llist \<Rightarrow> 'f set \<times> 'f set \<times> 'f set"
+where
+  "Liminf_zl_fstate Sts =
+   (Liminf_llist (lmap (passive.elems \<circ> passive_of) Sts),
+    Liminf_llist (lmap (set_option \<circ> yy_of) Sts),
+    Liminf_llist (lmap (fset \<circ> active_of) Sts))"
+
+
+subsection \<open>Initial States and Invariants\<close>
+
+inductive is_initial_fair_ZL_state :: "('t, 'p, 'f) fair_ZL_state_wo_ghosts \<Rightarrow> bool" where
+  "flat_inferences_of (set \<iota>ss) = no_labels.Inf_from {} \<Longrightarrow>
+   is_initial_fair_ZL_state (fold t_add \<iota>ss t_empty, p_empty, None, {||})"
+
+inductive fair_ZL_invariant :: "('t, 'p, 'f) fair_ZL_state_wo_ghosts \<Rightarrow> bool" where
+  "flat_inferences_of (todo.elems T) \<subseteq> Inf_F \<Longrightarrow> fair_ZL_invariant (T, P, Y, A)"
+
+
+subsection \<open>Completeness\<close>
 
 theorem
   assumes
-    full: "full_chain (\<leadsto>ZLf) Sts" and
+    full: "full_chain (\<leadsto>ZLfw) Sts" and
     init: "is_initial_fair_ZL_state (lhd Sts)" and
-    fair: "infinitely_often compute_infer_step Sts \<Longrightarrow> infinitely_often choose_p_step Sts" and
+    fair: "infinitely_often compute_infer_step Sts \<Longrightarrow>
+      infinitely_often choose_p_step Sts" and
     bot: "B \<in> Bot_F" and
     unsat: "passive.elems (passive_of (lhd Sts)) \<Turnstile>\<inter>\<G> {B}"
   shows
